@prefix dc: <http://purl.org/dc/elements/1.1/> .
@prefix dcterms: <http://purl.org/dc/terms/> .
@prefix rdf: <http://www.w3.org/1999/02/22-rdf-syntax-ns#> .
@prefix rdfs: <http://www.w3.org/2000/01/rdf-schema#> .
@prefix skos: <http://www.w3.org/2004/02/skos/core#> .
@prefix xml: <http://www.w3.org/XML/1998/namespace> .
@prefix xsd: <http://www.w3.org/2001/XMLSchema#> .

<http://purl.org/dcx/lrmi-vocabs/alignmentType/> a skos:ConceptScheme ;
    dc:description "Describes the types of relationships between a learning resource and an AlighmentObject."@en ;
    dc:title "LRMI Alignment Type Vocabulary"@en .

<http://purl.org/dcx/lrmi-vocabs/alignmentType/AT001> a skos:Concept ;
    skos:inScheme <http://purl.org/dcx/lrmi-vocabs/alignmentType/> ;
    skos:prefLabel "assesses"@en ;
    skos:definition "The learning resource may be used to assess the destination of the association." .

<http://purl.org/dcx/lrmi-vocabs/alignmentType/AT002> a skos:Concept ;
    skos:inScheme <http://purl.org/dcx/lrmi-vocabs/alignmentType/> ;
    skos:prefLabel "teaches"@en ;
    skos:definition "The learning resource may be used to teach the competency at the destination of the association." .

<http://purl.org/dcx/lrmi-vocabs/alignmentType/AT003> a skos:Concept ;
    skos:inScheme <http://purl.org/dcx/lrmi-vocabs/alignmentType/> ;
    skos:prefLabel "requires"@en ;
    skos:definition "The learning resource requires the destination of the association to support its function, delivery, or coherence." .

<http://purl.org/dcx/lrmi-vocabs/alignmentType/AT004> a skos:Concept ;
    skos:inScheme <http://purl.org/dcx/lrmi-vocabs/alignmentType/> ;
    skos:prefLabel "text complexity"@en ;
    skos:definition "The destination of the association defines a level or range, measuring the ease in which text can be read and understood, for text used within the learning resource." .

<http://purl.org/dcx/lrmi-vocabs/alignmentType/AT005> a skos:Concept ;
    skos:inScheme <http://purl.org/dcx/lrmi-vocabs/alignmentType/> ;
    skos:prefLabel "reading level"@en ;
    skos:definition "The destination of the association defines a level or range of ability expected for a person using the learning resource." .

<http://purl.org/dcx/lrmi-vocabs/alignmentType/AT006> a skos:Concept ;
    skos:inScheme <http://purl.org/dcx/lrmi-vocabs/alignmentType/> ;
    skos:prefLabel "educational subject"@en ;
    skos:definition "The destination of the association defines a topic or subject from a controlled vocabulary." .

<http://purl.org/dcx/lrmi-vocabs/alignmentType/AT007> a skos:Concept ;
    skos:inScheme <http://purl.org/dcx/lrmi-vocabs/alignmentType/> ;
    skos:prefLabel "educational level"@en ;
    skos:definition "The destination of the association defines an education level from a controlled vocabulary." .
